theories/AlmostStlc/Compatibility.v
@@ -37,113 +37,139 @@ Definition comp_bind {Γ MR t1 t2}
 Definition interp_mrec_bodies {t Γ MR R} (bodies : denote_bodies_type Γ MR R R) (m : denote_comp_type t Γ (R :: MR)) 
            : denote_comp_type t Γ MR :=
   fun hyps => interp_mrec (bodies hyps) (m hyps).
-  
-(* 
 
-   Lemma that is typically true according to nick
-   e1 --> e1' => e1' <=j e2 => e1 <=(j+1) e2
+Lemma multi_step_vis_dep_inv E `{EncodedType E} R S U
+      (t : entree E R) (k1 : R -> entree E S) k2 n e (f : encodes e -> U) :
+  encodes e = U ->
+  JMeq f (@id U) ->
+  multi_step n (vv <- t;; k1 vv) (vv <- (Vis e (fun x => Ret (f x)));; k2 vv) -> 
+  (exists (j1 j2 : nat) r, j1 + j2 = n /\ multi_step j1 t (ret r) /\
+                             multi_step j2 (k1 r) (vv <- (Vis e (fun x => Ret (f x)));; k2 vv)) \/
+  (exists k1', multi_step n t (vv <- (Vis e (fun x => Ret (f x)));; k1' vv) /\
+            forall vv1, vv2 <- k1' vv1;; k1 vv2 ≅ k2 vv1).
+Proof.
+  intros He Hid Hn. setoid_rewrite bind_vis in Hn.
+  eapply multi_step_vis_bind_inv in Hn.
+  destruct Hn as [[j1 [j2 [r [Hj [Hstep1 Hstep2]]]]] | [k1' [Hstep Heq] ] ].
+  - left. exists j1, j2, r. do 2 (split; auto). setoid_rewrite bind_vis. auto.
+  - right. setoid_rewrite bind_ret_l in Heq. subst. exists k1'. split; auto.
+    unfold id in *. setoid_rewrite bind_vis.
+    enough (Vis e k1' ≅ Vis e (fun x : encodes e => EnTree.bind (Ret x) (fun vv : encodes e => k1' vv))).
+    rewrite <- H0. auto. apply eqit_Vis. intros. rewrite bind_ret_l. reflexivity.
+Qed.
 
-   think about if this makes sense, especially in light of
-   whether you decrement steps in the ret case 
 
-*)
+Lemma multi_step_call_term_bind_inv T1 T2 MR R tin tout (xR : var R MR) (x : var (tin, tout) R) vvin 
+      (t : mtree (denote_mfix_ctx MR) T1) (k1 : T1 -> mtree (denote_mfix_ctx MR) T2) k2 n :
+  multi_step n (vv <- t;; k1 vv) (vv <- call_term x xR vvin;; k2 vv) -> 
+  (exists (j1 j2 : nat) (r : T1), j1 + j2 = n /\ multi_step j1 t (ret r) /\ multi_step j2 (k1 r) (vv <- call_term x xR vvin;; k2 vv)) \/
+  (exists k1', multi_step n t (vv <- call_term x xR vvin;; k1' vv) /\ forall vv1, vv2 <- k1' vv1;; k1 vv2 ≅ k2 vv1).
+Proof.
+  unfold call_term. destruct (call_mrec x xR vvin) as [d f] eqn : Heqx.
+  intros Hn. 
+  setoid_rewrite bind_trigger in Hn. setoid_rewrite bind_trigger. 
+  eapply multi_step_vis_dep_inv in Hn; eauto.
+  - specialize call_mrec_encodes with (xt := x) (xR := xR) (c := vvin). 
+    rewrite Heqx. auto.
+  - specialize call_mrec_cont with (xt := x) (xR := xR) (c := vvin). 
+    rewrite Heqx. auto.
+Qed.
 
-
+(*
 (* this might need to be an inductive proof *)
 Lemma let_compat Γ MR t1 t2 
       (m1 : denote_comp_type t1 Γ MR) (m2 : denote_comp_type t2 (t1 :: Γ) MR)
       (c1 : comp t1 Γ MR) (c2 : comp t2 (t1 :: Γ) MR)
   : comp_rel m1 c1 -> comp_rel m2 c2 ->
     comp_rel (comp_bind m1 m2) (comp_let c1 c2).
+*)
+Lemma let_compat_aux n : forall Γ MR t1 t2
+      (m1 : denote_comp_type t1 Γ MR) (m2 : denote_comp_type t2 (t1 :: Γ) MR)
+      (c1 : comp t1 Γ MR) (c2 : comp t2 (t1 :: Γ) MR),
+    bounded_comp_rel n m1 c1 -> bounded_comp_rel n m2 c2 ->
+    bounded_comp_rel n (comp_bind m1 m2) (comp_let c1 c2).
 Proof.
-  intros Hmc1 Hmc2. intros n hyps ρ Hhρ.
-  constructor. intros Hn. specialize (Hmc1 n hyps ρ Hhρ) as Hmc1n.
-  inversion Hmc1n. intros. subst. destruct (H Hn) as [Hretmc1 Hstuckmc1]. clear H.
+  induction n as [ n' IHn' ] using (well_founded_induction lt_wf).
+  intros ? ? ? ? ? ? ? ? Hmc1 Hmc2 n hyps ρ Hn' Hhρ.
+  (* can I just make this inductive? *)
+  constructor. intros j Hj. specialize (Hmc1 n hyps ρ Hn' Hhρ) as Hmc1n.
+  inversion Hmc1n. subst. rename H into Happrox1.
   split.
   - intros vv2 Hvv2. unfold comp_bind in Hvv2.
-    assert (exists vv1, comp_equiv_rutt (m1 hyps) (ret vv1)).
-    admit.
-    destruct H as [vv1 Hvv1]. specialize (Hretmc1 vv1 Hvv1).
+    eapply multi_step_ret_bind_inv in Hvv2.
+    destruct Hvv2 as [j1 [j2 [vv1 [Hn [Hvv11 Hvv12] ]]]].
+    (* problem here, look into it tomorrow, might be introducing *)
+    assert (Hj1 : j1 < n). lia.
+    specialize (Happrox1 j1 Hj1). destruct Happrox1 as [Hretmc1 _].
+    specialize (Hretmc1 vv1 Hvv11).
     destruct Hretmc1 as [v1 [Hv11 Hv12]].
-    (* maybe steps should not decrement in the ret case? 
-       I am concerned that might break other things  *) 
-    assert (Hhρ' : closing_subst_approx n (t1 :: Γ) (vv1, hyps) (v1, ρ)).
+    assert (Hhρ' : closing_subst_approx (n - j1) (t1 :: Γ) (vv1, hyps) (v1, ρ)).
     constructor; auto.
-    assert (comp_equiv_rutt (m2 (vv1, hyps)) (ret vv2)).
-    admit.
-    specialize (Hmc2 n (vv1, hyps) (v1, ρ) Hhρ') as Hmc2n.
-    inversion Hmc2n. 
-    destruct (H0 Hn) as [Hretmc2 Hstuckmc2]. clear H0.
-    apply Hretmc2 in H.
-    destruct H as [v2 [Hv21 Hv22]]. exists v2. split; auto.
-    admit.
+    destruct j1. assert (n - 0 = n). lia. rewrite H. auto.
+    eapply lower_closing_subst_approx; eauto. lia.
+    assert (Hnj1 : n - j1 <= n'). lia.
+    specialize (Hmc2 (n - j1) (vv1, hyps) (v1, ρ) Hnj1 Hhρ') as Hmc2n.
+    inversion Hmc2n. assert (Hj2 : j2 < n - j1). lia.
+    specialize (H j2 Hj2). destruct H as [Hretmc2 _ ].
+    specialize (Hretmc2 _ Hvv12). destruct Hretmc2 as [v2 [Hv21 Hv22]].
+    exists v2. split.
+    + (* need stepping metatheory, can be a focus next week *) admit.
+    + assert (n - j = n - j1 - j2). lia. rewrite H. auto.
   - intros. rename H into Hcall.
-    (* start tomorrow by stating this lemma assertion  *)
-    assert (Hcase :
-             (exists k', comp_equiv_rutt (m1 hyps) (vv <- call_term x xR vvcall;; k' vv))
-               \/
-             (exists vv1, comp_equiv_rutt (m1 hyps) (ret vv1) /\ 
-                       comp_equiv_rutt (m2 (vv1, hyps)) (vv <- call_term x xR vvcall;; k vv)
-           )).
-    admit.
-    destruct Hcase as [[k' Hk'] | [vv1 [Hvv11 Hvv12] ]].
-    + apply Hstuckmc1 in Hk' as Hcall'.
-      destruct Hcall' as [vcall [E [c' [Hvcall [HE1 [HE2 HE3 ]] ]]] ].
-       (* figure out how to construct the evaluation context that is morally this
-          perhaps close_comp is not general enough 
-          needs to be a more general substitution?
+    eapply multi_step_call_term_bind_inv in Hcall.
+    destruct Hcall as [[j1 [j2 [vv1 [Hj12 [Hstep1 Hstep2]] ]]] |  [k1' [Hstep Hk1']] ].
+    + assert (Hj1 : j1 < n). lia. specialize (Happrox1 j1 Hj1).
+      destruct Happrox1 as [Hretmc1 _]. specialize (Hretmc1 _ Hstep1).
+      destruct Hretmc1 as [v1 [Hstepv Happroxvv1]].
+      assert (Hhρ' : closing_subst_approx (n - j1) (t1 :: Γ) (vv1, hyps) (v1, ρ)).
+      constructor; auto.
+      destruct j1. assert (n - 0 = n). lia. rewrite H. auto.
+      eapply lower_closing_subst_approx; eauto. lia.
+      assert (Hnj1 : n - j1 <= n'). lia.
+      specialize (Hmc2 (n - j1) (vv1, hyps) (v1, ρ) Hnj1 Hhρ').
+      inversion Hmc2. subst.  assert (Hj2 : j2 < n - j1). lia.
+      specialize (H j2 Hj2). destruct H as [_ Hstuckmc2]. clear Hmc2.
+      apply Hstuckmc2 in Hstep2.
+      destruct Hstep2 as [vcall [E [c' [Hvcall [HE1 [HE2 HE3 ]] ]]] ].
+      exists vcall, E, c'.
+      split; [| split]; [| | split]; eauto.
+      * assert (H : n - j1 - j2 = n - (j1 + j2)). lia. rewrite <- H.
+        auto.
+      * admit. (* stepping metatheory *)
+      * intros. eapply HE3; eauto. lia.
+    + specialize (Happrox1 j Hj). destruct Happrox1 as [_ Hstuckmc1].
+      apply Hstuckmc1 in Hstep.
+       destruct Hstep as [vcall [E [c' [Hvcall [HE1 [HE2 HE3 ]] ]]] ].
+       exists vcall. eexists. eexists. (* comp_let c' c2 with proper closing*) 
+       split; [ | split]; [| | split]; eauto.
+       * admit. (* will require stepping metatheory *)
+       * admit. (* should be trivial once I can formalize the eval context 
+                  morally (ev_let E (close_comp Γ ρ c2)). but requires *)
+       * intros. rewrite <- Hk1'. clear Hstuckmc1.
+         assert (Hj'' : j'' < n'). lia.
+         specialize (IHn' j'' Hj'' [] MR t1 t2 (fun _ => k1' vvret) (fun '(vv2,_) => m2 (vv2, hyps))).
+         specialize (IHn' (subst_eval_context E (comp_ret vret))).
+         unfold comp_bind in IHn'. admit.
+         (* the choice of c2 requires an open substitution thing, but should be fine*)
 
-          morally
-          exists (ev_let E (close_comp Γ ρ c2)).
-
-          need a substitution that uses ρ to turn c2 into
-          a comp t2 [t1] MR,
-
-          then I need theorems about the order of substitutions 
-
-          there is a lot of ugly theory about closing substitutions I need
-
-        *) 
-      eexists.  eexists. eexists. split; eauto. split; [ | split]; eauto.
-      * admit.
-      * admit.
-      * intros. apply HE3 in H0; auto. 
-        (* concerned about this part 
-           k vvret = k' vvret ;; m2 kyps
-           use that to substitute in
-           if I have an induction hypothesis according to <
-           then maybe I can continue
-           this is starting to look sketchy, but not necessarily unsalvageable
-
-           also might be easier and sufficient to prove approx_comp composes with
-           bind/let at a fixed j'
-
-
-           should reduce/rewrite to 
-           (vv1 <- k' vvret;; m2 (vv1, hyps)) <=j' (
-              let (E[vret]]) (close ρ c2)
-
-
-              and by H0 we know k' vvret <=j' E[vret] (for this specific j')
-              and by Hmc2 we know forall j, m2 (vv1, hyps) <=j (close ρ c2)
-           
-
-         *)
-        admit.
-   + apply Hretmc1 in Hvv11 as Hvv13. destruct Hvv13 as [v1 [Hv11 Hv12]].
-     (* lost the thread a bit on this one *)
-     assert (Hhρ' : closing_subst_approx n (t1 :: Γ) (vv1, hyps) (v1, ρ)).
-     constructor; auto. specialize (Hmc2 _ _ _ Hhρ').
-     inversion Hmc2. specialize (H Hn). destruct H as [Hretmc2 Hstuckmc2].
-     subst. apply Hstuckmc2 in Hvv12 as Hvv13.
-     destruct Hvv13 as [vcall [E [c' [Hvcall [HE1 [HE2 HE3 ]] ]]] ].
-     exists vcall. eexists. eexists. split; [ auto | split ]; [ | split].
-     * admit.
-     * admit.
-     * auto.
-Admitted.
+         (* lots of details up in the air but this feels good *)
+         (* let Γ = [], m2 := fun vv2 => m2 (vv2, hyps), which I have knowledge about at j''*)
+         (* lets try to *)
+         (* I have info about k1' vvret at j'' or lower *)
+         (* I have infor about m2 at any level I have info about return of k1' vvret 
+            which is at most j'' *)
+         (* seems to fit with *)
+ Admitted.
 
 
+Lemma let_compat Γ MR t1 t2 
+      (m1 : denote_comp_type t1 Γ MR) (m2 : denote_comp_type t2 (t1 :: Γ) MR)
+      (c1 : comp t1 Γ MR) (c2 : comp t2 (t1 :: Γ) MR)
+  : comp_rel m1 c1 -> comp_rel m2 c2 ->
+    comp_rel (comp_bind m1 m2) (comp_let c1 c2).
+Proof.
+  intros. red. intros. eapply let_compat_aux; try red; eauto.
+Qed.
 
 Lemma mfix_compat t Γ R MR dbodies sbodies m (c : comp t Γ (R :: MR)):
   bodies_rel dbodies sbodies ->
@@ -152,7 +178,39 @@ Lemma mfix_compat t Γ R MR dbodies sbodies m (c : comp t Γ (R :: MR)):
 Proof.
   intros Hbodies Hmc n hyps ρ Hhρ.
   constructor. intros. split.
-  - intros vv Hvv. apply recursion_trace_den_ret in Hvv.
+  - intros vv Hvv. apply recursion_trace_ret in Hvv as Hvv'.
+    destruct Hvv' as [l Hrec].
+    specialize (Hmc n _ _ Hhρ).
+    (**)
+    unfold interp_mrec_bodies in Hvv.
+    generalize dependent (m hyps). generalize dependent c.
+    clear m.
+    (*Hhρ is a little problematic, could get rid of it if I can commute close_comp with 
+      comp_mfix *)
+    (* will require a bind lemma *)
+    induction j' as [ j IHj ] using (well_founded_induction lt_wf).
+    intros c m Happrox Hstep Hrec. dependent destruction Hrec.
+    + admit.
+    + admit.
+    +
+    
+    revert Happrox Hstep.
+    dependent induction Hrec.
+    + intros. setoid_rewrite H2 in Hstep. 
+      inversion Happrox. subst. assert (0 < n). lia. specialize (H0 0 H1).
+      destruct H0 as [Hret _].
+      setoid_rewrite H2 in Hret. assert (r = vv). apply eqit_Ret_inv in H3. subst. auto.
+      subst. specialize (Hret vv). 
+      assert (multi_step (E := denote_mrec_ctx (denote_mfix_ctx (R :: MR))) 0 (ret vv) (ret vv)).
+      constructor. reflexivity. specialize (Hret H0).
+      destruct Hret as [v [Hv1 Hv2]]. exists v.
+      split.
+      * (*step metatheory*) admit.
+      * destruct n0; auto. eapply lower_approx_val; try apply Hv2. lia.
+    + exfalso. (* ret ≅ vis*) admit.
+    +
+
+
     destruct Hvv as [l Hrec]. 
     assert (approx_comp (n + length l) approx_val (m hyps) (close_comp Γ ρ c)).
     apply Hmc. 
